pure/Learn.Option.fst
@@ -1,6 +1,7 @@
 module Learn.Option
 
 module U = Learn.Util
+module L = FStar.List.Pure
 
 noextract
 let opt_eq (#a : Type) (eq_a : U.eq_dec a) : U.eq_dec (option a)
@@ -18,3 +19,25 @@ let bind #a #b (x : option a) (f : a -> option b) : option b
   = match x with
   | None   -> None
   | Some x -> f x
+
+
+let rec traverse_list (#a : Type) (l : list (option a))
+  : Tot (option (list a)) (decreases l)
+  = match l with
+  | [] -> Some []
+  | (Some x) :: xs -> map (Cons x) (traverse_list xs)
+  | None :: _ -> None
+
+let rec traverse_list_length (#a : Type) (l : list (option a))
+  : Lemma (requires Some? (traverse_list l)) (ensures L.length (Some?.v (traverse_list l)) == L.length l)
+          [SMTPat (traverse_list l)]
+  = match l with
+  | [] -> ()
+  | Some _ :: xs -> traverse_list_length xs
+
+let rec traverse_list_index (#a : Type) (l : list (option a)) (i : Fin.fin (L.length l))
+  : Lemma (requires Some? (traverse_list l))
+          (ensures  Some? (L.index l i) /\ L.index (Some?.v (traverse_list l)) i == Some?.v (L.index l i))
+  = match l with
+  | [] -> ()
+  | Some _ :: xs -> if i > 0 then traverse_list_index xs (i-1)
