experiment/Experiment.Steel.Tac.LV.fst
@@ -1,0 +1,320 @@
+module Experiment.Steel.Tac.LV
+
+module U    = Learn.Util
+module L    = FStar.List.Pure
+module M    = Experiment.Steel.Repr.M
+module Ll   = Learn.List
+module Veq  = Experiment.Steel.VEquiv
+module Opt  = Learn.Option
+module Perm = Learn.Permutation
+
+open Experiment.Steel.VPropList
+open Learn.List.Mask
+open Experiment.Steel.Repr.LV
+open FStar.Tactics
+open Learn.Tactics.Util
+open Experiment.Steel.Interface
+open Experiment.Steel.Tac
+
+
+(**** Building a [eq_injection_l] *)
+
+let traverse_partial_injection
+      (#a : Type) (src trg : list a)
+      (ij : Veq.partial_injection src trg)
+  : Lemma (requires Some? (Opt.traverse_list ij))
+          (ensures  is_eq_injection src trg (L.index (Some?.v (Opt.traverse_list ij))))
+  =
+    let ij' = L.index (Some?.v (Opt.traverse_list ij)) in
+    Perm.injectiveI ij' (fun i i' ->
+      Opt.traverse_list_index ij i;
+      Opt.traverse_list_index ij i');
+    introduce forall (i : Fin.fin (L.length src)) . L.index trg (ij' i) == L.index src i
+      with Opt.traverse_list_index ij i
+
+[@@ __cond_solver__]
+let __build_eq_injection_l
+      (#a : Type) (src trg : list a)
+      (ij0 : Veq.partial_injection src trg)
+      (ij1 : list (Fin.fin (L.length trg)))
+      (ij1_eq : squash (Some ij1 == Opt.traverse_list ij0))
+  : eq_injection_l src trg
+  =
+    (**) traverse_partial_injection src trg ij0;
+    ij1
+
+let __normal_build_eq_injection_l : list norm_step = [
+  delta_only [`%L.splitAt; `%L.length; `%Ll.initi; `%len; `%Ll.set;
+              `%Opt.traverse_list; `%Opt.map];
+  delta_attr [`%__cond_solver__];
+  iota; zeta; primops
+]
+
+/// Solves a goal [eq_injection_l src trg].
+let build_eq_injection_l fr ctx : Tac unit
+  =
+    let goal = cur_goal () in
+    apply_raw (`__build_eq_injection_l);
+    // ij0
+    build_partial_injection fr ctx;
+    // ij1
+    dismiss (); //ij1
+    norm __normal_build_eq_injection_l;
+    cs_try trefl fr ctx (fun m -> fail (m Fail_eq_injection [Info_goal goal]))
+    // TODO better error message: show remaining elements
+
+let test_build_eq_injection_l
+  : eq_injection_l (String.list_of_string "aabc") (String.list_of_string "faedcab")
+  = _ by (norm [primops]; build_eq_injection_l default_flags dummy_ctx)
+
+
+(**** Building a [Perm.pequiv_list] *)
+
+let eq_injection_pequiv_list
+      (#a : Type) (src trg : list a)
+      (ij : eq_injection_l src trg)
+  : Lemma (requires L.length trg == L.length src)
+          (ensures  src == Perm.apply_perm_r (Perm.perm_f_of_list ij) trg)
+  = Ll.list_extensionality src (Perm.apply_perm_r (Perm.perm_f_of_list ij) trg) (fun i -> ())
+
+[@@ __cond_solver__]
+let __build_pequiv_list
+      (#a : Type) (src trg : list a)
+      (eq_len : squash L.(length trg == length src))
+      (ij : eq_injection_l src trg)
+  : Perm.pequiv_list trg src
+  =
+    (**) eq_injection_pequiv_list src trg ij;
+    ij
+
+/// Solves a goal [Perm.pequiv_list l0 l1]
+let build_pequiv_list fr ctx : Tac unit
+  =
+    apply (`__build_pequiv_list);
+    // eq_len
+    cs_try (fun () ->
+      norm [delta_only [`%L.length]; iota; zeta; primops];
+      trefl ()
+    ) fr ctx (fun m -> fail (m Fail_pequiv_len []));
+    // ij
+    build_eq_injection_l fr ctx
+
+let test_build_pequiv_list
+  : Perm.pequiv_list (String.list_of_string "aabc") (String.list_of_string "caba")
+  = _ by (norm [primops]; build_pequiv_list default_flags dummy_ctx)
+
+
+(*** Building a [lin_cond] *)
+
+// TODO? propagate a partial [prd]
+
+let __normal_lc : list norm_step = [
+  delta_only [`%L.map; `%L.length; `%Ll.initi; `%L.mem; `%L.op_At; `%L.append; `%L.splitAt;
+              `%Mktuple2?._1; `%Mktuple2?._2];
+  delta_attr [`%__cond_solver__; `%__lin_cond__; `%__mask__];
+  iota; zeta; primops
+]
+
+let norm_lc () : Tac unit =
+  norm __normal_lc
+
+
+#push-options "--fuel 0 --ifuel 0"
+
+[@@ __cond_solver__]
+let lcsub_add_csm
+      (env : vprop_list) (#a : Type) (t : M.prog_tree a)
+      (csm0 : csm_t env) (prd0 : prd_t a)
+      (lc : lin_cond env t csm0 prd0)
+      (csm1 : csm_t env) (prd1 : prd_t a)
+      (prd1_f : (x : a) -> Perm.pequiv_list
+                L.(prd0 x @ filter_mask (mask_diff csm0 csm1) (filter_mask (mask_not csm0) env))
+                (prd1 x))
+  : lin_cond env t (mask_comp_or csm0 (mask_diff csm0 csm1)) prd1
+  =
+    let csm' = mask_diff csm0 csm1 in
+    LCsub env csm0 prd0 lc csm' prd1 prd1_f
+
+/// [LCret] with [prd = sl_hint]
+[@@ __cond_solver__]
+let __build_LCret
+      (env : vprop_list)
+      (a : Type u#a) (x : a) (sl_hint : M.post_t a)
+      (csm_f : eq_injection_l (sl_hint x) env)
+  : lin_cond env (M.Tret a x sl_hint) (eij_trg_mask csm_f) sl_hint
+  = LCret env #a #x #sl_hint sl_hint csm_f
+
+[@@ __cond_solver__]
+let __build_LCbind
+      (env : vprop_list)
+      (a : Type u#a) (b : Type u#a) (f : M.prog_tree a) (g : (a -> M.prog_tree b))
+      (f_csm : csm_t env) (f_prd : prd_t a)
+      (cf : lin_cond env f f_csm f_prd)
+      (g_csm0 : (x : a) -> csm_t (res_env env f_csm (f_prd x))) (g_prd0 : (x : a) -> prd_t b)
+      (cg : (x : a) -> lin_cond (res_env env f_csm (f_prd x)) (g x) (g_csm0 x) (g_prd0 x))
+      (g_csm : csm_t (filter_mask (mask_not f_csm) env)) (g_prd : prd_t b)
+      (eqs : (x : a) -> squash (
+            let n0 = L.length (f_prd x) in
+            L.splitAt_length n0 (g_csm0 x);
+            let m : Ll.vec n0 bool = (L.splitAt n0 (g_csm0 x))._1 in
+            let add = filter_mask (mask_not m) (f_prd x) in
+            eq2 #(list bool) g_csm (L.splitAt (L.length (f_prd x)) (g_csm0 x))._2 /\
+            g_prd == (fun (y : b) -> L.(g_prd0 x y @ add))))
+  : lin_cond env (M.Tbind a b f g) (bind_csm env f_csm g_csm) g_prd
+  =
+    LCbind env #a #b #f #g
+      f_csm f_prd cf
+      g_csm g_prd
+      (fun (x : a) ->
+        let env1 = res_env env f_csm (f_prd x) in
+        let n0 = L.length (f_prd x)            in
+        let n1 = mask_len (mask_not f_csm)     in
+        L.splitAt_length n0 (g_csm0 x);
+        let g_csm0a, g_csm0b = L.splitAt n0 (g_csm0 x) in
+        let g_csm0a : Ll.vec n0 bool = g_csm0a in
+        let g_csm0b : Ll.vec n1 bool = g_csm0b in
+        Ll.lemma_splitAt_append n0 (g_csm0 x);
+        assert (g_csm0 x == L.(g_csm0a @ g_csm0b));
+
+        let g_csm1 = mask_split_l n0 n1 in
+
+        let g_csm_0 = mask_comp_or (g_csm0 x) (mask_diff (g_csm0 x) g_csm1) in
+        let g_csm_1 = bind_g_csm' env f_csm (f_prd x) g_csm                 in
+        Ll.list_extensionality g_csm_0 g_csm_1
+          (fun i ->
+            Ll.pat_append ();
+            if i >= n0 then begin
+              assert (L.index g_csm_0 i == L.index (g_csm0 x) i);
+              calc (==) {
+                L.index g_csm_1 i;
+              == { }
+                L.index g_csm (i-n0);
+              == { eqs x }
+                L.index g_csm0b (i - n0);
+              == { L.lemma_splitAt_reindex_right n0 (g_csm0 x) (i - n0) }
+                L.index (g_csm0 x) i;
+              }
+            end);
+
+        lcsub_add_csm env1 (g x) (g_csm0 x) (g_prd0 x) (cg x) g_csm1 g_prd
+          (fun (y : b) ->
+            calc (==) {
+              g_prd y;
+            == { eqs x }
+              L.(g_prd0 x y @ filter_mask (mask_not g_csm0a) (f_prd x));
+            };
+            calc (==) {
+              filter_mask (mask_diff (g_csm0 x) g_csm1) (filter_mask (mask_not (g_csm0 x)) env1) <: vprop_list;
+            == { filter_mask_diff_comm (g_csm0 x) g_csm1 env1 }
+              filter_mask (filter_mask g_csm1 (mask_not (g_csm0 x))) (filter_mask g_csm1 env1);
+            == { }
+              filter_mask (mask_not (filter_mask g_csm1 L.(g_csm0a @ g_csm0b)))
+                          (filter_mask g_csm1 L.(f_prd x @ filter_mask (mask_not f_csm) env));
+            == { filter_mask_split_l n0 n1 g_csm0a g_csm0b;
+                 filter_mask_split_l n0 n1 (f_prd x) (filter_mask (mask_not f_csm) env) }
+              filter_mask (mask_not g_csm0a) (f_prd x);
+            };
+            Perm.perm_f_to_list (Perm.pequiv_refl (g_prd y))))
+#pop-options
+
+[@@ __cond_solver__]
+let __defer_sig_unification
+      (#env : vprop_list) (#a : Type) (#t : M.prog_tree a)
+      (#csm0 : csm_t env) (#prd0 : prd_t a)
+      (lc : lin_cond env t csm0 prd0)
+      (#csm1 : csm_t env) (#prd1 : prd_t a)
+      (_ : squash (csm1 == csm0 /\ prd1 == prd0))
+  : lin_cond env t csm1 prd1
+  = lc
+
+/// The following tactics solve goals of the form [lin_cond env t ?csm ?prd]
+
+let build_LCspec fr : Tac unit
+  =
+    apply (`LCspec);
+    build_eq_injection_l fr (fun () -> [Info_location "before the spec statement"])
+
+let build_LCret fr : Tac unit
+  =
+    apply (`__build_LCret);
+    build_eq_injection_l fr (fun () -> [Info_location "at the return statement"])
+
+let rec build_LCbind fr : Tac unit
+  =
+    apply (`__build_LCbind);
+    // cf
+    build_lin_cond fr;
+    // cg
+    let x = intro () in
+    norm_lc ();
+    build_lin_cond fr;
+    // [g_csm <- ...], [g_prd <- ...]
+    let x = intro () in
+    norm_lc ();
+    split ();
+      let ctx () = [Info_location "in the bind statement"] in
+      cs_try trefl fr ctx (fun m -> fail (m (Fail_dependency "csm" x) []));
+      cs_try trefl fr ctx (fun m -> fail (m (Fail_dependency "prd" x) []))
+
+and build_lin_cond fr : Tac unit
+  =
+    let build_tac : flags_record -> Tac unit =
+      let goal = cur_goal () in
+      let args = (collect_app goal)._2 in
+      let fail_shape () =
+        cs_raise fr dummy_ctx (fun m -> fail (m (Fail_goal_shape GShape_lin_cond) [Info_goal goal])) in
+      if L.length args <> 5
+      then fail_shape ()
+      else let hd = (collect_app (L.index args 2)._1)._1 in
+      match inspect hd with
+      | Tv_FVar fv | Tv_UInst fv _ ->
+          // TODO? better solution to match
+          let nd = inspect_fv fv in
+          if Nil? nd then (let _ = fail_shape () in fail "unreachable");
+          begin match L.last nd with
+          | "Tspec"  -> build_LCspec
+          | "TspecS" -> fail "TODO"
+          | "Tret"   -> build_LCret
+          | "Tbind"  -> build_LCbind
+          | "TbindP" -> fail "TODO"
+          | "Tif"    -> fail "TODO"
+          | _ -> fail_shape ()
+          end
+      | r -> fail_shape ()
+    in
+    // changes [lin_cond env t ?csm0 ?prd0]
+    // into [lin_cond env t ?csm1 ?prd1] and [?csm0 = ?csm1 /\ ?prd0 = ?prd1]
+    // where [?csm1] and [?prd1] are fresh uvars
+    apply (`__defer_sig_unification);
+    // solves [lin_cond env t ?csm1 ?prd1], instantiate [?csm1] and [?prd1]
+    build_tac fr;
+    // [?csm0 <- csm1], [?prd0 <- prd1]
+    norm_lc ();
+    split (); trefl (); trefl ()
+
+#push-options "--ifuel 0 --fuel 0"
+[@@ __cond_solver__]
+let __build_top_lin_cond
+      (#a : Type) (t : M.prog_tree a) (pre : vprop_list) (post : M.post_t a)
+      (csm0 : csm_t pre) (prd0 : prd_t a)
+      (lc : lin_cond pre t csm0 prd0)
+      (veq : (x : a) -> Perm.pequiv_list L.(prd0 x @ filter_mask (mask_not csm0) pre) (post x))
+  : top_lin_cond t pre post
+  =
+    (**) Ll.list_extensionality (mask_comp_or csm0 (mask_diff csm0 (csm_all pre))) (csm_all pre) (fun i -> ());
+    lcsub_add_csm pre t csm0 prd0 lc (csm_all pre) post
+      (fun x ->
+        (**) filter_mask_true (mask_diff csm0 (csm_all pre)) (filter_mask (mask_not csm0) pre) (fun i -> ());
+        veq x)
+#pop-options
+
+/// Solves a goal [top_lin_cond t pre post]
+let build_top_lin_cond fr : Tac unit
+  =
+    apply (`__build_top_lin_cond);
+    // lc
+    build_lin_cond fr;
+    // veq
+    let x = intro () in
+    norm_lc ();
+    build_pequiv_list fr (fun () -> [Info_location "at the end of the program"])
