experiment/Experiment.Steel.Tac.Test.fst
@@ -4,17 +4,18 @@ module M    = Experiment.Steel.Repr.M
 module U    = Learn.Util
 module L    = FStar.List.Pure
 module Ll   = Learn.List
+module LV   = Experiment.Steel.Repr.LV
 module Fin  = FStar.Fin
 module Perm = Learn.Permutation
 
 open FStar.Tactics
 open Learn.Tactics.Util
+open Experiment.Steel.VPropList
 open Steel.Effect
 open Steel.FractionalPermission
 open Steel.Reference
 open Experiment.Steel.Interface
 open Experiment.Steel.Tac
-open Experiment.Steel.Tac.MCond
 
 
 let test_flags = make_flags_record [Full_Msg]
@@ -47,6 +48,10 @@ let norm_test () : Tac unit
           delta_qualifier ["unfold"];
           iota; zeta; primops]
 
+
+(*** MCond *)
+
+open Experiment.Steel.Tac.MCond
 
 let test_TCspec_u (v0 v1 : vprop') : squash True =
   _ by (let post' = fresh_uvar (Some (`(M.post_t int))) in
@@ -334,3 +339,82 @@ let test_build_tree_cond__smt_fallback_0 (r0 r1 : ref int)
         (M.Tret unit () (fun _ -> []))
         [vptr' r0 full_perm] (fun _ -> [vptr' r1 full_perm])
   = _ by (let _ = build_tree_cond test_flags true in ())
+
+
+(*** LV *)
+
+open Experiment.Steel.Tac.LV
+
+noeq
+type lin_cond_r (env : vprop_list) (#a : Type) (t : M.prog_tree a) = {
+  lcr_csm : LV.csm_t env;
+  lcr_prd : LV.prd_t a;
+  lcr_lc  : LV.lin_cond env t lcr_csm lcr_prd
+}
+
+let test_LCspec (v0 v1 : vprop') (vx0 : int -> vprop')
+  : lin_cond_r [v0; v1] (specT int [v0] (fun x -> [vx0 x]))
+  = _ by (
+    norm_test (); apply (`Mklin_cond_r);
+    build_LCspec test_flags
+  )
+
+let test_LCret (v0 v1 : vprop') (vx0 : int -> vprop')
+  : lin_cond_r [v0; v1; vx0 0] (M.Tret int 0 (fun x -> [v1; vx0 x]))
+  = _ by (
+    norm_test (); apply (`Mklin_cond_r);
+    build_LCret test_flags
+  )
+
+let test_LCbind (v0 v1 v2 v3 : vprop') (vx0 vx1 : int -> vprop')
+  : lin_cond_r [v0; v1; v2] (M.Tbind int int (specT int [v0] (fun x -> [v3; vx0 x]))
+                                   (fun x -> specT int [vx0 x; v1] (fun y -> [vx1 y])))
+  = _ by (
+    norm_test (); apply (`Mklin_cond_r);
+    build_LCbind test_flags
+  )
+
+let test_lin_cond0 (v : int -> vprop') (vx : int -> int -> vprop')
+  : LV.top_lin_cond
+      (M.Tbind int int (specT int [v 0] (fun x -> [v 3; vx 0 x]))
+             (fun x -> specT int [vx 0 x; v 1] (fun y -> [vx 1 y])))
+      [v 0; v 1; v 2] (fun y -> [v 3; vx 1 y; v 2])
+  = _ by (norm_test (); build_top_lin_cond test_flags)
+
+let test_lin_cond1 (v : vprop') (vx : int -> vprop')
+  : LV.top_lin_cond
+      (M.Tbind int int (M.Tret int 0 (fun x -> [vx x]))
+             (fun x -> M.Tret int x (fun x -> [vx x])))
+      [v; vx 0] (fun x -> [v; vx x])
+  = _ by (build_top_lin_cond test_flags)
+
+/// Contrary to [Tac.MCond] we do not propagate the post when it is known so [sl_hint] is always needed when a [Tret]
+/// introduces a dependency.
+[@@ expect_failure [228]]
+let test_lin_cond__ret_hint0 (vx : int -> vprop')
+  : LV.top_lin_cond
+      (M.Tret int 0 (fun _ -> []))
+      [vx 0] (fun x -> [vx x])
+  = _ by (build_top_lin_cond test_flags)
+
+let test_lin_cond__ret_hint1 (vx : int -> vprop')
+  : LV.top_lin_cond
+      (M.Tret int 0 (fun x -> [vx x]))
+      [vx 0] (fun x -> [vx x])
+  = _ by (build_top_lin_cond test_flags)
+
+
+[@@ expect_failure [228]]
+let test_lin_cond__fail0 (v : int -> vprop')
+  : LV.top_lin_cond
+      (M.Tret int 0 (fun _ -> [v 1]))
+      [v 0] (fun _ -> [v 1])
+  = _ by (build_top_lin_cond test_flags)
+
+[@@ expect_failure [228]]
+let test_lin_cond__fail1 (vx : int -> vprop')
+  : LV.top_lin_cond
+      (M.Tbind int int (specT int [] (fun x -> [vx x]))
+             (fun x -> M.Tret int 0 (fun _ -> [])))
+      [] (fun x -> [])
+  = _ by (norm_test (); build_top_lin_cond test_flags)
